bedrock2/src/Map/SeparationLogic.v
@@ -1,12 +1,11 @@
 Require Import Coq.Classes.Morphisms.
 Require Import bedrock2.Map bedrock2.Map.Decomp bedrock2.Lift1Prop bedrock2.Map.Separation. Import map.
+Require Coq.Lists.List.
 
 Section SepProperties.
   Context {key value} {map : map key value} {ok : ok map}.
   Local Infix "*" := sep.
 
-  Global Instance Proper_emp_iff : Proper (iff ==> iff1) emp. firstorder idtac. Qed.
-  Global Instance Proper_emp_impl : Proper (Basics.impl ==> impl1) emp. firstorder idtac. Qed.
   Global Instance Proper_sep_iff1 : Proper (iff1 ==> iff1 ==> iff1) sep. firstorder idtac. Qed.
   Global Instance Proper_sep_impl1 : Proper (impl1 ==> impl1 ==> impl1) sep. firstorder idtac. Qed.
 
@@ -25,14 +24,35 @@ Section SepProperties.
   Proof. cbv [iff1 sep split]; t; eauto 10 using union_comm, (fun m1 m2 => proj2 (disjoint_comm m1 m2)). Qed.
   Lemma sep_assoc p q r : iff1 ((p*q)*r) (p*(q*r)).
   Proof. cbv [iff1 sep split]; t; eauto 15 using eq_sym, union_assoc, ((fun m1 m2 m3 => proj2 (disjoint_union_l m1 m2 m3))), ((fun m1 m2 m3 => proj2 (disjoint_union_r m1 m2 m3))). Qed.
-  Lemma sep_213 B A C : iff1 (A * (B * C)) (B * (A * C)).
-  Proof. rewrite <-(sep_assoc _ B), (sep_comm _ B), sep_assoc. reflexivity. Qed.
 
-  (* sep and ex1 *)
-  Lemma sep_ex1_r {T} p (q:T->_) : iff1 (p * ex1 q) (ex1 (fun h => p * q h)).
-  Proof. firstorder idtac. Qed.
-  Lemma sep_ex1_l {T} p (q:T->_) : iff1 (ex1 q * p) (ex1 (fun h => q h * p)).
-  Proof. rewrite sep_comm. rewrite sep_ex1_r. setoid_rewrite (sep_comm p). reflexivity. Qed.
+  Lemma get_ptsto k v m (H : ptsto k v m) : get m k = Some v.
+  Proof. rewrite H, get_put_same; trivial. Qed.
+  Lemma get_sep k v R m (H : sep (ptsto k v) R m) : get m k = Some v.
+  Proof.
+    destruct H as (mk&mR&H&Hp&HR); eapply get_ptsto in Hp; subst.
+    destruct (get_split k _ _ _ H) as [[]|[]]; congruence.
+  Qed.
+  Lemma sep_put (key_eq_dec : forall k1 k2 : key, k1 = k2 \/ k1 <> k2)
+        k v m v_old R (H : sep (ptsto k v_old) R m) : sep (ptsto k v) R (put m k v).
+  Proof.
+    eapply sep_comm in H; eapply sep_comm.
+    destruct H as (mR&mk&[Heq Hd]&HR&Hp); cbv [ptsto] in Hp; subst mk; subst m.
+    exists mR, (put empty k v); split; [|solve[repeat split; trivial]]; split.
+    { eapply map_ext; intro k'; destruct (key_eq_dec k' k); try subst k';
+        rewrite ?get_put_same, ?get_put_diff by trivial.
+      { erewrite get_union_right; trivial. rewrite get_put_same; trivial. }
+      { rewrite 2get_union_left; trivial. all:rewrite get_put_diff, get_empty; trivial. } }
+    { intros k' ? ? ? Hget; intros; destruct (key_eq_dec k' k); try subst k'.
+      { eapply Hd; eauto using get_put_same. }
+      { rewrite get_put_diff, get_empty in Hget by trivial; inversion Hget. } }
+  Qed.
+
+  Lemma iff1_sep_cancel P Q1 Q2 (H : iff1 Q1 Q2) : iff1 (P * Q1) (P * Q2).
+  Proof. exact (Proper_sep_iff1 _ _ (reflexivity _) _ _ H). Qed.
+
+  (* More Conntectives *)
+  Global Instance Proper_emp_iff : Proper (iff ==> iff1) emp. firstorder idtac. Qed.
+  Global Instance Proper_emp_impl : Proper (Basics.impl ==> impl1) emp. firstorder idtac. Qed.
 
   (* sep and emp *)
   Lemma sep_emp_emp p q : iff1 (sep (emp p) (emp q)) (emp (p /\ q)).
@@ -42,12 +62,6 @@ Section SepProperties.
   Proof. rewrite <-sep_assoc. rewrite (sep_comm a). rewrite sep_assoc. reflexivity. Qed.
   Lemma sep_emp_12 a b c : iff1 (emp a * (emp b * c)) (emp (a /\ b) * c).
   Proof. rewrite <-sep_assoc. rewrite sep_emp_emp. reflexivity. Qed.
-
-  (* impl1 and emp *)
-  Lemma impl1_l_sep_emp (a:Prop) b c : impl1 (emp a * b) c <-> (a -> impl1 b c).
-  Proof. cbv [impl1 emp sep split]; t; rewrite ?union_empty_l; eauto 10 using union_empty_l, disjoint_empty_l. Qed.
-  Lemma impl1_r_sep_emp a b c : (b /\ impl1 a c) -> impl1 a (emp b * c).
-  Proof. cbv [impl1 emp sep split]; t; eauto 10 using union_empty_l, disjoint_empty_l. Qed.
 
   Lemma sep_emp_l a b m : sep (emp a) b m <-> a /\ b m.
   Proof.
@@ -62,24 +76,62 @@ Section SepProperties.
     setoid_rewrite sep_comm || (etransitivity; [eapply sep_comm|]). (* WHY? *)
     eapply sep_emp_l.
   Qed.
-End SepProperties.
+  Lemma sep_emp_True_l p : iff1 (sep (emp True) p) p.
+  Proof. intros m; rewrite sep_emp_l; intuition idtac. Qed.
+  Lemma sep_emp_True_r p : iff1 (sep p (emp True)) p.
+  Proof. intros m; rewrite sep_emp_r; intuition idtac. Qed.
 
-Ltac set_evars := repeat match goal with |- context[?e] => is_evar e; set e end.
-Ltac subst_evars := repeat match goal with x := ?e |- _ => is_evar e; subst x end.
-Ltac normalize :=
-  set_evars;
-  (* COQBUG? Why is the repeat necessary? Why does it not work inside rewrite_strat? *)
-  repeat (rewrite_strat (bottomup (terms @sep_emp_emp @sep_comm_emp_r @sep_emp_12 @sep_emp_2 @sep_ex1_l @sep_ex1_r @sep_assoc)));
-  subst_evars.
-Ltac cancel_atom_goal1 P :=
-  (* COQBUG: if I use fresh here, rewrite_strat fails *)
-  pose proof (sep_213 P) as __PRIVATE_cancel_atom_goal1_ASDA;
-  (rewrite_strat (try (bottomup (terms __PRIVATE_cancel_atom_goal1_ASDA))));
-  clear __PRIVATE_cancel_atom_goal1_ASDA.
-Ltac cancel_atom P :=
-  eapply Proper_impl1_impl1; [ cbv [Basics.flip]; cancel_atom_goal1 P; eapply (Proper_sep_impl1 P _ (reflexivity _)) | reflexivity | reflexivity ].
-Ltac cancel :=
-  lazymatch goal with |- impl1 _ (sep _ _) => idtac end;
-  set_evars;
-  repeat match goal with |- impl1 _ (sep ?P _) => cancel_atom P end;
-  subst_evars.
+  (* sep and ex1 *)
+  Lemma sep_ex1_r {T} p (q:T->_) : iff1 (p * ex1 q) (ex1 (fun h => p * q h)).
+  Proof. firstorder idtac. Qed.
+  Lemma sep_ex1_l {T} p (q:T->_) : iff1 (ex1 q * p) (ex1 (fun h => q h * p)).
+  Proof. rewrite sep_comm. rewrite sep_ex1_r. setoid_rewrite (sep_comm p). reflexivity. Qed.
+
+  (* impl1 and emp *)
+  Lemma impl1_l_sep_emp (a:Prop) b c : impl1 (emp a * b) c <-> (a -> impl1 b c).
+  Proof. cbv [impl1 emp sep split]; t; rewrite ?union_empty_l; eauto 10 using union_empty_l, disjoint_empty_l. Qed.
+  Lemma impl1_r_sep_emp a b c : (b /\ impl1 a c) -> impl1 a (emp b * c).
+  Proof. cbv [impl1 emp sep split]; t; eauto 10 using union_empty_l, disjoint_empty_l. Qed.
+
+  (* seps *)
+  Fixpoint seps' (xs : list (rep -> Prop)) : rep -> Prop :=
+    match xs with
+    | cons x xs => sep x (seps' xs)
+    | nil => emp True
+    end.
+  Lemma seps'_iff1_seps xs : iff1 (seps' xs) (seps xs).
+  Proof.
+    induction xs; [exact (reflexivity _)|].
+    destruct xs; [solve[eauto using sep_emp_True_r]|].
+    eapply Proper_sep_iff1, IHxs.
+    exact (reflexivity _).
+  Qed.
+
+  Let nth n xs := List.hd (emp True) (List.skipn n xs).
+  Let remove_nth n (xs : list (rep -> Prop)) :=
+    (List.firstn n xs ++ List.tl (List.skipn n xs))%list.
+  Lemma seps_nth_to_head n xs : iff1 (sep (nth n xs) (seps (remove_nth n xs))) (seps xs).
+  Proof.
+    cbv [nth remove_nth].
+    pose proof (List.firstn_skipn n xs).
+    set (xsr := List.skipn n xs) in *; clearbody xsr.
+    set (xsl := List.firstn n xs) in *; clearbody xsl.
+    subst xs.
+    setoid_rewrite <-seps'_iff1_seps.
+    destruct xsr.
+    { cbn [seps']; rewrite sep_emp_True_l, 2List.app_nil_r; exact (reflexivity _). }
+    cbn [List.hd List.tl].
+    induction xsl; cbn; [exact (reflexivity _)|].
+    rewrite <-IHxsl; clear IHxsl.
+    rewrite (sep_comm _ (seps' _)), <-(sep_assoc _ (seps' _)), <-(sep_comm _ (_ * seps' _)).
+    exact (reflexivity _).
+  Qed.
+  Lemma cancel_seps_at_indices i j xs ys
+        (Hij : iff1 (nth i xs) (nth j ys))
+        (Hrest : iff1 (seps (remove_nth i xs)) (seps (remove_nth j ys)))
+    : iff1 (seps xs) (seps ys).
+  Proof.
+    rewrite <-(seps_nth_to_head i xs), <-(seps_nth_to_head j ys), Hij, Hrest.
+    exact (reflexivity _).
+  Qed.
+End SepProperties.
